external/Goose/github_com/mit_pdos/tulip/quorum.v
@@ -16,35 +16,4 @@ Definition Half: val :=
   rec: "Half" "n" :=
     ("n" + #1) `quot` #2.
 
-Definition swap: val :=
-  rec: "swap" "ns" "i" "j" :=
-    let: "tmp" := SliceGet uint64T "ns" "i" in
-    SliceSet uint64T "ns" "i" (SliceGet uint64T "ns" "j");;
-    SliceSet uint64T "ns" "j" "tmp";;
-    #().
-
-Definition sort: val :=
-  rec: "sort" "ns" :=
-    let: "i" := ref_to uint64T #1 in
-    Skip;;
-    (for: (λ: <>, (![uint64T] "i") < (slice.len "ns")); (λ: <>, Skip) := λ: <>,
-      let: "j" := ref_to uint64T (![uint64T] "i") in
-      Skip;;
-      (for: (λ: <>, (![uint64T] "j") > #0); (λ: <>, Skip) := λ: <>,
-        (if: (SliceGet uint64T "ns" ((![uint64T] "j") - #1)) ≤ (SliceGet uint64T "ns" (![uint64T] "j"))
-        then Break
-        else
-          swap "ns" ((![uint64T] "j") - #1) (![uint64T] "j");;
-          "j" <-[uint64T] ((![uint64T] "j") - #1);;
-          Continue));;
-      "i" <-[uint64T] ((![uint64T] "i") + #1);;
-      Continue);;
-    #().
-
-(* NB: Follow the proof of wrbuf.sortEntsByKey *)
-Definition Median: val :=
-  rec: "Median" "ns" :=
-    sort "ns";;
-    SliceGet uint64T "ns" ((slice.len "ns") `quot` #2).
-
 End code.
