external/Goose/github_com/mit_pdos/tulip/util.v
@@ -14,4 +14,29 @@ Definition NextAligned: val :=
     else "delta" <-[uint64T] (("interval" + "low") - "rem"));;
     std.SumAssumeNoOverflow "current" (![uint64T] "delta").
 
+Definition swap: val :=
+  rec: "swap" "ns" "i" "j" :=
+    let: "tmp" := SliceGet uint64T "ns" "i" in
+    SliceSet uint64T "ns" "i" (SliceGet uint64T "ns" "j");;
+    SliceSet uint64T "ns" "j" "tmp";;
+    #().
+
+Definition Sort: val :=
+  rec: "Sort" "ns" :=
+    let: "i" := ref_to uint64T #1 in
+    Skip;;
+    (for: (λ: <>, (![uint64T] "i") < (slice.len "ns")); (λ: <>, Skip) := λ: <>,
+      let: "j" := ref_to uint64T (![uint64T] "i") in
+      Skip;;
+      (for: (λ: <>, (![uint64T] "j") > #0); (λ: <>, Skip) := λ: <>,
+        (if: (SliceGet uint64T "ns" ((![uint64T] "j") - #1)) ≤ (SliceGet uint64T "ns" (![uint64T] "j"))
+        then Break
+        else
+          swap "ns" ((![uint64T] "j") - #1) (![uint64T] "j");;
+          "j" <-[uint64T] ((![uint64T] "j") - #1);;
+          Continue));;
+      "i" <-[uint64T] ((![uint64T] "i") + #1);;
+      Continue);;
+    #().
+
 End code.
