src/program_proof/tulip/paxos/program/paxos.v
@@ -1,8 +1,11 @@
 From Perennial.program_proof.tulip.paxos Require Import prelude.
 From Perennial.program_proof.tulip.paxos.invariance Require Import
   accept advance ascend commit extend prepare.
-From Perennial.program_proof.tulip.util Require Import next_aligned.
+From Perennial.program_proof.tulip.program.util Require Import next_aligned sort.
+From Perennial.program_proof.tulip.program Require Import quorum.
 From Goose.github_com.mit_pdos.tulip Require Import paxos.
+
+(* Local Ltac Zify.zify_post_hook ::= Z.div_mod_to_equations. *)
 
 Section repr.
   Context `{!heapGS Σ, !paxos_ghostG Σ}.
@@ -67,11 +70,10 @@ Section repr.
   (*@     conns     map[uint64]grove_ffi.Connection                           @*)
   (*@ }                                                                       @*)
   Definition own_paxos_comm (paxos : loc) (peers : gset u64) : iProp Σ :=
-    ∃ (peersP : Slice.t) (addrpeersP : loc) (connsP : loc),
-      "HpeersP"     ∷ paxos ↦[Paxos :: "peers"] (to_val peersP) ∗
+    ∃ (me : u64) (addrpeersP : loc) (connsP : loc),
+      "HmeP"        ∷ paxos ↦[Paxos :: "me"] #me ∗
       "HaddrpeersP" ∷ paxos ↦[Paxos :: "addrpeers"] #addrpeersP ∗
-      "HconnsP"     ∷ paxos ↦[Paxos :: "conns"] #connsP ∗
-      "#Hpeers"     ∷ own_slice peersP uint64T DfracDiscarded (elements peers).
+      "HconnsP"     ∷ paxos ↦[Paxos :: "conns"] #connsP.
 
   Definition own_paxos_candidate_only
     (nidme termc terml termp : u64) (logc : list string)
@@ -86,42 +88,72 @@ Section repr.
       "%Hpltc"    ∷ ⌜uint.Z termp < uint.Z termc⌝.
 
   Definition own_paxos_candidate
-    (paxos : loc) (nid termc terml : u64) (entsc : list string) (iscand : bool) nids γ : iProp Σ :=
+    (paxos : loc) (nid termc terml : u64) (logc : list string) (iscand : bool) nids γ : iProp Σ :=
     ∃ (termp : u64) (entspP : Slice.t) (resppP : loc),
       "HiscandP" ∷ paxos ↦[Paxos :: "iscand"] #iscand ∗
       "HtermpP"  ∷ paxos ↦[Paxos :: "termp"] #termp ∗
       "HentspP"  ∷ paxos ↦[Paxos :: "entsp"] (to_val entspP) ∗
       "HresppP"  ∷ paxos ↦[Paxos :: "respp"] #resppP ∗
       "Honlyc"   ∷ (if iscand
-                    then own_paxos_candidate_only nid termc terml termp entsc entspP resppP nids γ
+                    then own_paxos_candidate_only nid termc terml termp logc entspP resppP nids γ
                     else True).
 
+  Definition accepted_or_committed_until γ nids nid (a : bool) t n : iProp Σ :=
+    if a
+    then is_accepted_proposal_length_lb γ nid t n
+    else (∃ v, safe_ledger_above γ nids t v ∗ ⌜length v = n⌝)%I.
+
+  #[global]
+  Instance accepted_or_committed_until_persistent γ nids nid a t n :
+    Persistent (accepted_or_committed_until γ nids nid a t n).
+  Proof. destruct a; apply _. Defined.
+
+  Definition safe_peer_lsns γ nids t (lsns : gmap u64 u64) : iProp Σ :=
+    ∃ (aocm : gmap u64 bool),
+      ([∗ map] nid ↦ i; a ∈ lsns; aocm,
+         accepted_or_committed_until γ nids nid a t (uint.nat i)).
+
   Definition own_paxos_leader_only
-    (termc : u64) (log : list string) (lsnpeersP : loc) γ : iProp Σ :=
+    (termc terml : u64) (log : list string) (lsnpeersP : loc) (peers : gset u64)
+    nids γ : iProp Σ :=
     ∃ (lsnpeers : gmap u64 u64),
       "Hps"        ∷ own_proposal γ (uint.nat termc) log ∗
       "Hlsnpeers"  ∷ own_map lsnpeersP (DfracOwn 1) lsnpeers ∗
-      "#Hpfb"      ∷ prefix_base_ledger γ (uint.nat termc) log ∗
-      "%Hlelenlog" ∷ ⌜map_Forall (λ _ i, (uint.nat i ≤ length log)%nat) lsnpeers⌝.
+      "#Haocm"     ∷ safe_peer_lsns γ nids (uint.nat termc) lsnpeers ∗
+      "%Hleqc"     ∷ ⌜terml = termc⌝ ∗
+      "%Hlelog"    ∷ ⌜map_Forall (λ _ i, (uint.nat i ≤ length log)%nat) lsnpeers⌝ ∗
+      "%Hinclnids" ∷ ⌜dom lsnpeers ⊆ peers⌝.
 
   Definition own_paxos_leader
-    (paxos : loc) (termc : u64) (log : list string) (isleader : bool) γ : iProp Σ :=
+    (paxos : loc) (termc terml : u64) (log : list string) (isleader : bool) (peers : gset u64)
+    nids γ : iProp Σ :=
     ∃ (lsnpeersP : loc),
       "HisleaderP" ∷ paxos ↦[Paxos :: "isleader"] #isleader ∗
       "HlsnpeersP" ∷ paxos ↦[Paxos :: "lsnpeers"] #lsnpeersP ∗
-      "Honlyl"     ∷ (if isleader then own_paxos_leader_only termc log lsnpeersP γ else True).
+      "Honlyl"     ∷ (if isleader
+                      then own_paxos_leader_only termc terml log lsnpeersP peers nids γ
+                      else True).
 
   Definition own_paxos_sc (paxos : loc) (nids : gset u64) : iProp Σ :=
     ∃ (sc : u64),
-      "HscP" ∷ paxos ↦[Paxos :: "sc"] #sc ∗
-      "%Hsc" ∷ ⌜size nids = uint.nat sc⌝.
-  
+      "HscP"    ∷ paxos ↦[Paxos :: "sc"] #sc ∗
+      (* This condition allows a nicer implementation and proof for pushing the
+      committed LSN (i.e., @px.push). *)
+      "%Hmulti" ∷ ⌜1 < uint.Z sc⌝ ∗
+      "%Hsc"    ∷ ⌜size nids = uint.nat sc⌝.
+
+  Definition own_paxos_nids
+    (paxos : loc) (nidme : u64) (peers : gset u64) nids : iProp Σ :=
+    ∃ (peersP : Slice.t),
+      "HnidmeP"  ∷ paxos ↦[Paxos :: "nidme"] #nidme ∗
+      "HpeersP"  ∷ paxos ↦[Paxos :: "peers"] (to_val peersP) ∗
+      "Hpeers"   ∷ own_slice peersP uint64T (DfracOwn 1) (elements peers) ∗
+      "%Hnids"   ∷ ⌜nids = {[nidme]} ∪ peers⌝ ∗
+      "%Hnidsne" ∷ ⌜nidme ∉ peers⌝.
+
   Definition own_paxos_common
-    (paxos : loc) (nidme termc terml lsnc : u64) (log : list string)
-    (nids : gset u64) γ : iProp Σ :=
-    ∃ (me : u64) (hb : bool) (logP : Slice.t) (peers : gset u64),
-      "HmeP"     ∷ paxos ↦[Paxos :: "me"] #me ∗
-      "HnidP"    ∷ paxos ↦[Paxos :: "nidme"] #nidme ∗
+    (paxos : loc) (nidme termc terml lsnc : u64) (log : list string) nids γ : iProp Σ :=
+    ∃ (hb : bool) (logP : Slice.t),
       "HhbP"     ∷ paxos ↦[Paxos :: "hb"] #hb ∗
       "HtermcP"  ∷ paxos ↦[Paxos :: "termc"] #termc ∗
       "Htermc"   ∷ own_current_term_half γ nidme (uint.nat termc) ∗
@@ -131,14 +163,13 @@ Section repr.
       "Hlog"     ∷ own_slice logP stringT (DfracOwn 1) log ∗
       "Hlogn"    ∷ own_node_ledger_half γ nidme log ∗
       "HlsncP"   ∷ paxos ↦[Paxos :: "lsnc"] #lsnc ∗
-      "Hcomm"    ∷ own_paxos_comm paxos peers ∗
       "Hsc"      ∷ own_paxos_sc paxos nids ∗
+      "#Hgebase" ∷ prefix_base_ledger γ (uint.nat terml) log ∗
       "#Hpreped" ∷ (if decide (termc = terml)
                     then True
                     else past_nodedecs_latest_before γ nidme (uint.nat termc) (uint.nat terml) log) ∗
       "#Hacpted" ∷ is_accepted_proposal_lb γ nidme (uint.nat terml) log ∗
       "#Hcmted"  ∷ safe_ledger_above γ nids (uint.nat terml) (take (uint.nat lsnc) log) ∗
-      "%Hnids"   ∷ ⌜nids = {[nidme]} ∪ peers⌝ ∗
       "%Hnid"    ∷ ⌜0 ≤ uint.Z nidme < max_nodes⌝ ∗
       "%Htermlc" ∷ ⌜uint.Z terml ≤ uint.Z termc⌝ ∗
       "%Hlsncub" ∷ ⌜uint.Z lsnc ≤ length log⌝.
@@ -150,11 +181,13 @@ Section repr.
   predicates should be existentially quantified. *)
   Definition own_paxos_internal
     (paxos : loc) (nidme termc terml lsnc : u64) (iscand isleader : bool) nids γ : iProp Σ :=
-    ∃ (log : list string),
+    ∃ (log : list string) (peers : gset u64),
       let logc := (take (uint.nat lsnc) log) in
       "Hpx"     ∷ own_paxos_common paxos nidme termc terml lsnc log nids γ ∗
       "Hcand"   ∷ own_paxos_candidate paxos nidme termc terml logc iscand nids γ ∗
-      "Hleader" ∷ own_paxos_leader paxos termc log isleader γ.
+      "Hleader" ∷ own_paxos_leader paxos termc terml log isleader peers nids γ ∗
+      "Hnids"   ∷ own_paxos_nids paxos nidme peers nids ∗
+      "Hcomm"   ∷ own_paxos_comm paxos peers.
 
   Definition own_paxos_with_termc_lsnc
     (paxos : loc) (nidme termc lsnc : u64) nids γ : iProp Σ :=
@@ -184,6 +217,11 @@ Section repr.
   Definition own_paxos_with_termc_terml
     (paxos : loc) (nidme termc terml : u64) nids γ : iProp Σ :=
     ∃ (lsnc : u64) (iscand : bool) (isleader : bool),
+      own_paxos_internal paxos nidme termc terml lsnc iscand isleader nids γ.
+
+  Definition own_paxos_with_termc_terml_iscand
+    (paxos : loc) (nidme termc terml : u64) (iscand : bool) nids γ : iProp Σ :=
+    ∃ (lsnc : u64) (isleader : bool),
       own_paxos_internal paxos nidme termc terml lsnc iscand isleader nids γ.
 
   Definition own_paxos (paxos : loc) (nidme : u64) nids γ : iProp Σ :=
@@ -223,7 +261,7 @@ Section stepdown.
     (*@     px.iscand = false                                                   @*)
     (*@     px.isleader = false                                                 @*)
     (*@                                                                         @*)
-    do 2 iNamed "Hpx". iNamed "Hcand". iNamed "Hleader".
+    do 2 iNamed "Hpx". iNamed "Hcand". iNamed "Hleader". iNamed "Hnids".
     do 3 wp_storeField.
 
     (*@     // TODO: Write @px.termc to disk.                                   @*)
@@ -270,7 +308,7 @@ Section nominate.
     (*@     px.termc = term                                                     @*)
     (*@     px.isleader = false                                                 @*)
     (*@                                                                         @*)
-    do 2 iNamed "Hpx". iNamed "Hleader".
+    do 2 iNamed "Hpx". iNamed "Hleader". iNamed "Hnids".
     do 2 wp_loadField.
     wp_apply wp_NextAligned.
     { word. }
@@ -465,6 +503,27 @@ Section inv.
       by iApply (node_inv_past_nodedecs_impl_prefix_base_ledger with "Hdslb Hnode").
     }
     by iApply (safe_ledger_prefix_base_ledger_impl_prefix with "Hsafe Hpfb Hinv").
+  Qed.
+
+  Lemma accepted_proposal_growing_proposal_impl_prefix γ nids nid t v1 v2 :
+    nid ∈ nids ->
+    is_accepted_proposal_lb γ nid t v1 -∗
+    own_proposal γ t v2 -∗
+    paxos_inv γ nids -∗
+    ⌜prefix v1 v2⌝.
+  Proof.
+    iIntros (Hinnids) "Hv1 Hv2 Hinv".
+    iNamed "Hinv".
+    rewrite -Hdomtermlm elem_of_dom in Hinnids.
+    destruct Hinnids as [terml Hterml].
+    iDestruct (big_sepM_lookup with "Hnodes") as "Hnode"; first apply Hterml.
+    iNamed "Hnode".
+    iDestruct (accepted_proposal_prefix with "Hv1 Hpsa") as %(vub1 & Hvub1 & Hprefix1).
+    iDestruct (big_sepM_lookup with "Hpsaubs") as (vub2) "[Hvub2 %Hprefix2]"; first apply Hvub1.
+    iDestruct (proposal_prefix with "Hvub2 Hv2") as %Hprefix.
+    iPureIntro.
+    trans vub1; first done.
+    by trans vub2.
   Qed.
 
 End inv.
@@ -855,6 +914,7 @@ Section ascend.
 
     (*@     // Logical action: Ascend(@px.termc, @px.log).                      @*)
     (*@                                                                         @*)
+    iNamed "Hnids".
     iInv "Hinv" as "> HinvO" "HinvC".
     iMod (paxos_inv_ascend with "[] Htermc Hterml Hlogn HinvO")
       as "(Htermc & Hterml & Hlogn & HinvO & Hps & #Hpsb & #Hacptlb)".
@@ -875,10 +935,15 @@ Section ascend.
     set logc := take (uint.nat lsnc) log.
     set log' := logc ++ entsp.
     set logc' := take (uint.nat lsnc) log'.
-    iAssert (own_paxos_leader px termc log' true γ)%I
+    iAssert (own_paxos_leader px termc termc log' true peers nids γ)%I
       with "[$HisleaderP $HlsnpeersP $Hlsnpeers $Hps]" as "Hleader".
+    { iSplit; last done.
+      iExists ∅.
+      by rewrite big_sepM2_empty.
+    }
+    iAssert (prefix_base_ledger γ (uint.nat termc) log')%I as "#Hpfb'".
     { by iFrame "Hpsb". }
-    iDestruct (safe_ledger_above_mono (uint.nat terml) logc' (uint.nat termc) with "[]")
+    iDestruct (safe_ledger_above_mono (uint.nat terml) (uint.nat termc) logc' with "[]")
       as "Hcmted'".
     { word. }
     { subst logc log' logc'.
@@ -888,13 +953,12 @@ Section ascend.
     }
     iClear "Hcmted".
     iFrame "Hleader".
-    iFrame "HtermcP HtermlP HiscandP".
+    iFrame "HtermcP HtermlP HiscandP Hpfb'".
     iFrame "∗ # %".
     iModIntro.
     iSplit.
     { iClear "Hpreped". by case_decide. }
     iPureIntro.
-    split; first done.
     split; first done.
     subst log'.
     rewrite length_app length_take.
@@ -1022,7 +1086,7 @@ Section accept.
         { iFrame "Hcand Hleader HlogP".
           by iFrame "∗ # %".
         }
-        iDestruct (safe_ledger_above_mono (uint.nat terml) logc (uint.nat term) with "Hcmted")
+        iDestruct (safe_ledger_above_mono (uint.nat terml) (uint.nat term) logc with "Hcmted")
           as "Hcmted'".
         { clear -Htermlc. word. }
         iFrame "Hcmted'".
@@ -1061,6 +1125,7 @@ Section accept.
 
       (*@         // Logical action: Advance(term, log).                          @*)
       (*@                                                                         @*)
+      iNamed "Hnids".
       iInv "Hinv" as "> HinvO" "HinvC".
       iMod (paxos_inv_advance with "Hpfb Hpfg Htermc Hterml Hlogn HinvO")
         as "(Htermc & Hterml & Hlogn & HinvO & #Hacpted')".
@@ -1091,7 +1156,7 @@ Section accept.
         by rewrite take_idemp.
       }
       iMod ("HinvC" with "HinvO") as "_".
-      iDestruct (safe_ledger_above_mono (uint.nat terml) logc' (uint.nat term) with "[]")
+      iDestruct (safe_ledger_above_mono (uint.nat terml) (uint.nat term) logc' with "[]")
         as "Hcmted'".
       { word. }
       { subst logc'.
@@ -1108,7 +1173,6 @@ Section accept.
         case_decide; last done.
         iFrame "∗ # %".
         iPureIntro.
-        split; first done.
         split; first done.
         rewrite -Heq.
         word.
@@ -1186,6 +1250,7 @@ Section accept.
       clear -Hszlog Hszents Hnogap Hlonger.
       word.
     }
+    iNamed "Hnids".
     iInv "Hinv" as "> HinvO" "HinvC".
     iMod (paxos_inv_accept with "Hpfb Hpfg Htermc Hterml Hlogn HinvO")
       as "(Htermc & Hterml & Hlogn & HinvO & #Hacpted')".
@@ -1217,7 +1282,6 @@ Section accept.
         clear -Hlsncub. word.
       }
       iPureIntro.
-      split; first done.
       apply prefix_length in Hprefix.
       clear -Hlsncub Hprefix.
       word.
@@ -1279,7 +1343,7 @@ Section obtain.
       by rewrite -Hszlog drop_all uint_nat_W64_0 /=.
     }
     apply map_get_true in Hok.
-    apply Hlelenlog in Hok.
+    apply Hlelog in Hok.
 
     (*@     // The follower has reported up to where the log is matched         @*)
     (*@     // (i.e., @lsne), so send everything after that.                    @*)
@@ -1310,6 +1374,498 @@ Section obtain.
   Qed.
 
 End obtain.
+
+Section forward.
+  Context `{!heapGS Σ, !paxos_ghostG Σ}.
+
+  Theorem wp_Paxos__forward
+    (px : loc) (nid lsn : u64) (nidme termc : u64) (loga : list string) nids γ :
+    nid ≠ nidme ->
+    nid ∈ nids ->
+    length loga = uint.nat lsn ->
+    (is_accepted_proposal_lb γ nid (uint.nat termc) loga ∨
+     safe_ledger_above γ nids (uint.nat termc) loga) -∗
+    know_paxos_inv γ nids -∗
+    {{{ own_paxos_leading_with_termc px nidme termc nids γ }}}
+      Paxos__forward #px #nid #lsn
+    {{{ RET #(); own_paxos_leading_with_termc px nidme termc nids γ }}}.
+  Proof.
+    iIntros (Hnotme Hnid Hlena) "#Haoc #Hinv".
+    iIntros (Φ) "!> Hpx HΦ".
+    wp_rec.
+
+    (*@ func (px *Paxos) forward(nid uint64, lsn uint64) {                      @*)
+    (*@     lsnpeer, ok := px.lsnpeers[nid]                                     @*)
+    (*@                                                                         @*)
+    iNamed "Hpx". iNamed "Hleader". iNamed "Honlyl".
+    subst terml.
+    wp_loadField.
+    wp_apply (wp_MapGet with "Hlsnpeers").
+    iIntros (lsnpeer ok) "[%Hok Hlsnpeers]".
+    wp_pures.
+
+    (*@     if !ok || lsnpeer < lsn {                                           @*)
+    (*@         // Advance the peer's matching LSN.                             @*)
+    (*@         px.lsnpeers[nid] = lsn                                          @*)
+    (*@     }                                                                   @*)
+    (*@ }                                                                       @*)
+    (* Not sure how to properly handle TC resolution here. *)
+    unshelve wp_apply (wp_or_pure (negb ok)).
+    { shelve. }
+    { apply _. }
+    { shelve. }
+    { wp_pures. by destruct ok; case_bool_decide. }
+    { iIntros (_). by  wp_pures. }
+    wp_if_destruct.
+    { wp_loadField.
+      wp_apply (wp_MapInsert with "Hlsnpeers"); first done.
+      iIntros "Hlsnpeers".
+      wp_pures.
+      iInv "Hinv" as "> HinvO" "HinvC".
+      iAssert (⌜(length loga ≤ length log)%nat⌝)%I as %Hle.
+      { iDestruct "Haoc" as "[Hacpted | Hcmted]".
+        { (* Case: [loga] is accepted by [nid]. *)
+          iDestruct (accepted_proposal_growing_proposal_impl_prefix with "Hacpted Hps HinvO")
+            as %Hprefix.
+          { apply Hnid. }
+          iPureIntro.
+          by apply prefix_length.
+        }
+        (* Case: [loga] has already be committed at this or an early term. *)
+        iDestruct "Hcmted" as (p) "[Hsafe %Hple]".
+        destruct (decide (p = uint.nat termc)) as [-> | Hne].
+        { (* Case: [loga] committed in the current term. *)
+          iDestruct "Hsafe" as (nidx) "Hsafe".
+          iNamed "Hsafe".
+          iDestruct (accepted_proposal_growing_proposal_impl_prefix with "Hvacpt Hps HinvO")
+            as %Hprefix.
+          { apply Hmember. }
+          iPureIntro.
+          by apply prefix_length.
+        }
+        (* Case: [loga] committed in an early term. *)
+        assert (Hlt : (p < uint.nat termc)%nat) by lia.
+        iNamed "Hpx".
+        iDestruct (safe_ledger_prefix_base_ledger_impl_prefix with "Hsafe Hgebase HinvO")
+          as %Hprefix.
+        { apply Hlt. }
+        iPureIntro.
+        by apply prefix_length.
+      }
+      iMod ("HinvC" with "HinvO") as "_".
+      iNamed "Hnids".
+      iApply "HΦ".
+      iFrame "Hpx Hcand".
+      iFrame "∗ #".
+      iModIntro.
+      iAssert (safe_peer_lsns γ nids (uint.nat termc) (<[nid := lsn]> lsnpeers))%I as "Haocm'".
+      { iDestruct "Haoc" as "[Hacpted | Hcmted]".
+        { iNamed "Haocm".
+          iExists (<[nid := true]> aocm).
+          iApply big_sepM2_insert_2; last done.
+          iFrame "Hacpted".
+          iPureIntro. lia.
+        }
+        { iNamed "Haocm".
+          iExists (<[nid := false]> aocm).
+          iApply big_sepM2_insert_2; last done.
+          iFrame "Hcmted".
+          iPureIntro. lia.
+        }
+      }
+      iFrame "Haocm'".
+      iPureIntro.
+      split; last set_solver.
+      split; first done.
+      split.
+      { apply map_Forall_insert_2; [lia | apply Hlelog]. }
+      { rewrite dom_insert_L. set_solver. }
+    }
+    iApply "HΦ".
+    iFrame "Hpx Hcand".
+    by iFrame "∗ # %".
+  Qed.
+
+End forward.
+
+Section commit.
+  Context `{!heapGS Σ, !paxos_ghostG Σ}.
+
+  Theorem wp_Paxos__commit
+    (px : loc) (lsn : u64) (nidme term : u64) (logc : list string) nids γ :
+    length logc = uint.nat lsn ->
+    safe_ledger_above γ nids (uint.nat term) logc -∗
+    know_paxos_inv γ nids -∗
+    {{{ own_paxos_with_termc_terml_iscand px nidme term term false nids γ }}}
+      Paxos__commit #px #lsn
+    {{{ RET #(); own_paxos_with_termc_terml_iscand px nidme term term false nids γ }}}.
+  Proof.
+    iIntros (Hlenlogc) "#Hsafe #Hinv".
+    iIntros (Φ) "!> Hpx HΦ".
+    wp_rec.
+
+    (*@ func (px *Paxos) commit(lsn uint64) {                                   @*)
+    (*@     if lsn <= px.lsnc {                                                 @*)
+    (*@         return                                                          @*)
+    (*@     }                                                                   @*)
+    (*@                                                                         @*)
+    do 2 iNamed "Hpx". iNamed "Hnids".
+    wp_loadField.
+    wp_if_destruct.
+    { iApply "HΦ".
+      iFrame "Hleader Hcand".
+      by iFrame "∗ # %".
+    }
+    rename Heqb into Hgtlsnc.
+    rewrite Z.nle_gt in Hgtlsnc.
+    iDestruct (own_slice_sz with "Hlog") as %Hszlog.
+    iApply fupd_wp.
+    iInv "Hinv" as "> HinvO" "HinvC".
+    iAssert (⌜prefix log logc ∨ prefix logc log⌝)%I as %Horprefix.
+    { iDestruct "Hsafe" as (p) "[Hsafe %Hple]".
+      destruct (decide (p = uint.nat term)) as [-> | Hne]; last first.
+      { iDestruct (safe_ledger_prefix_base_ledger_impl_prefix with "Hsafe Hgebase HinvO")
+          as %Hprefix.
+        { clear -Hple Hne. lia. }
+        iPureIntro.
+        by right.
+      }
+      iNamed "Hsafe".
+      iDestruct (paxos_inv_impl_nodes_inv_psa with "HinvO") as (bs) "[Hnodes %Hdombs]".
+      iApply (nodes_inv_is_accepted_proposal_lb_impl_prefix with "Hacpted Hvacpt Hnodes").
+      { set_solver. }
+      { by rewrite Hdombs. }
+    }
+    iMod ("HinvC" with "HinvO") as "_".
+    iModIntro.
+
+    (*@     if uint64(len(px.log)) < lsn {                                      @*)
+    (*@         px.lsnc = uint64(len(px.log))                                   @*)
+    (*@         return                                                          @*)
+    (*@     }                                                                   @*)
+    (*@                                                                         @*)
+    wp_loadField.
+    wp_apply wp_slice_len.
+    wp_if_destruct.
+    { rename Heqb into Hgtlog.
+      wp_loadField.
+      wp_apply wp_slice_len.
+      wp_storeField.
+      destruct Horprefix as [Hprefix | Hprefix]; last first.
+      { apply prefix_length in Hprefix. exfalso.
+        clear -Hgtlog Hprefix Hszlog Hlenlogc. word.
+      }
+      iApply "HΦ".
+      iFrame "Hcand Hleader".
+      iFrame "∗ # %".
+      iModIntro.
+      iSplit.
+      { rewrite -Hszlog firstn_all.
+        by iApply (safe_ledger_above_weaken log with "Hsafe").
+      }
+      iPureIntro.
+      clear -Hszlog. word.
+    }
+    rename Heqb into Hlelog.
+    rewrite Z.nlt_ge in Hlelog.
+
+    (*@     px.lsnc = lsn                                                       @*)
+    (*@                                                                         @*)
+    wp_storeField.
+    iApply "HΦ".
+    iFrame "Hcand Hleader".
+    iFrame "∗ # %".
+    iModIntro.
+    iSplit.
+    { assert (Hprefix : prefix logc log).
+      { destruct Horprefix as [Hprefix | ?]; last done.
+        rewrite (prefix_length_eq _ _ Hprefix); first done.
+        lia.
+      }
+      iApply (safe_ledger_above_weaken with "Hsafe").
+      by rewrite -Hlenlogc take_length_prefix.
+    }
+    iPureIntro.
+    clear -Hlelog Hszlog. word.
+
+    (*@     // TODO: Write @px.lsnc to disk.                                    @*)
+    (*@ }                                                                       @*)
+  Qed.
+
+End commit.
+
+Section push.
+  Context `{!heapGS Σ, !paxos_ghostG Σ}.
+
+  Theorem wp_Paxos__push (px : loc) (nidme termc : u64) nids γ :
+    know_paxos_inv γ nids -∗
+    {{{ own_paxos_leading_with_termc px nidme termc nids γ }}}
+      Paxos__push #px
+    {{{ (lsnc : u64) (ok : bool), RET (#lsnc, #ok);
+        own_paxos_leading_with_termc px nidme termc nids γ ∗
+        if ok
+        then ∃ logc, safe_ledger_above γ nids (uint.nat termc) logc ∗
+                     ⌜length logc = uint.nat lsnc⌝
+        else True
+    }}}.
+  Proof.
+    iIntros "#Hinv" (Φ) "!> Hpx HΦ".
+    wp_rec.
+
+    (*@ func (px *Paxos) push() (uint64, bool) {                                @*)
+    (*@     if !px.cquorum(uint64(len(px.lsnpeers)) + 1) {                      @*)
+    (*@         // Nothing should be done without responses from some quorum of nodes. @*)
+    (*@         return 0, false                                                 @*)
+    (*@     }                                                                   @*)
+    (*@                                                                         @*)
+    do 2 iNamed "Hpx". iNamed "Hleader". iNamed "Honlyl". iNamed "Hnids".
+    wp_loadField.
+    wp_apply (wp_MapLen with "Hlsnpeers").
+    iIntros "[%Hszlsnpeers Hlsnpeers]".
+    wp_apply (wp_Paxos__cquorum with "Hsc").
+    iIntros (ok) "[Hsc %Hqsize]".
+    (* Not using [wp_if_destruct] to prevent it eating equality about [nids]. *)
+    destruct ok eqn:Hok; last first.
+    { wp_pures.
+      iApply "HΦ".
+      iFrame "Hcand".
+      by iFrame "∗ # %".
+    }
+    
+    (*@     var lsns = make([]uint64, 0, px.sc)                                 @*)
+    (*@                                                                         @*)
+    iNamed "Hsc".
+    wp_loadField.
+    wp_apply wp_NewSliceWithCap.
+    { word. }
+    iIntros (lsnsinitP) "Hlsns".
+    wp_apply wp_ref_to; first done.
+    iIntros (lsnsPP) "HlsnsPP".
+
+    (*@     for _, lsn := range(px.lsnpeers) {                                  @*)
+    (*@         lsns = append(lsns, lsn)                                        @*)
+    (*@     }                                                                   @*)
+    (*@                                                                         @*)
+    wp_loadField.
+    rewrite uint_nat_W64_0 /=.
+    set P := (λ (m : gmap u64 u64), ∃ (lsnsP' : Slice.t) (lsns' : list u64),
+                 "HlsnsP" ∷ lsnsPP ↦[slice.T uint64T] (to_val lsnsP')  ∗
+          "Hlsns"   ∷ own_slice lsnsP' uint64T (DfracOwn 1) lsns' ∗
+          "%Hlsns'" ∷ ⌜(map_to_list m).*2 ≡ₚ lsns'⌝)%I.
+    wp_apply (wp_MapIter_fold _ _ _ P with "Hlsnpeers [$HlsnsPP $Hlsns]").
+    { set_solver. }
+    { (* Loop body. *)
+      clear Φ.
+      iIntros (m nid lsn Φ) "!> (HP & %Hnone & %Hlsn) HΦ".
+      iNamed "HP".
+      wp_load.
+      wp_apply (wp_SliceAppend with "Hlsns").
+      iIntros (lsnsP'') "Hlsns".
+      wp_store.
+      iApply "HΦ".
+      iFrame.
+      iPureIntro.
+      rewrite map_to_list_insert; last apply Hnone.
+      rewrite fmap_cons Hlsns' /=.
+      apply Permutation_cons_append.
+    }
+    iIntros "[Hlsnpeers HP]".
+    iNamed "HP". clear P.
+
+    (*@     util.Sort(lsns)                                                     @*)
+    (*@                                                                         @*)
+    wp_load.
+    wp_apply (wp_Sort with "Hlsns").
+    iIntros (lsnsorts) "(Hlsns & %Hsorted & %Hperm)".
+    wp_load.
+    wp_apply wp_slice_len.
+    wp_loadField.
+    wp_load.
+    iDestruct (own_slice_sz with "Hlsns") as %Hszsorted.
+    rewrite Hperm -Hlsns' length_fmap length_map_to_list in Hszsorted.
+    rewrite word.unsigned_add Hsc in Hqsize.
+    set i := word.sub _ _.
+    assert (is_Some (lsnsorts !! uint.nat i)) as [lsn Hlsn].
+    { apply lookup_lt_is_Some_2.
+      subst i.
+      rewrite Hperm -Hlsns' length_fmap length_map_to_list.
+      rewrite word.unsigned_sub_nowrap; last word.
+      word.
+    }
+    iDestruct (own_slice_to_small with "Hlsns") as "Hlsns".
+    wp_apply (wp_SliceGet with "[$Hlsns]").
+    { iPureIntro. apply Hlsn. }
+    iIntros "Hlsns".
+    wp_pures.
+
+    (*@     return lsn, true                                                    @*)
+    (*@ }                                                                       @*)
+    iApply "HΦ".
+    iModIntro.
+    iSplit.
+    { iFrame "Hcand".
+      by iFrame "∗ # %".
+    }
+    iDestruct (own_slice_sz with "Hlog") as %Hszlog.
+    set lsnpeersq := filter (λ x, (uint.nat lsn ≤ uint.nat x.2)%nat) lsnpeers.
+    set nidpeersq := dom lsnpeersq.
+    iDestruct "Haocm" as (aocm) "Haocm".
+    set aocmq := filter (λ x, x.1 ∈ nidpeersq) aocm.
+    destruct (decide (map_Exists (λ _ b, b = false) aocmq)) as [Hsomecmted | Hallacpted].
+    { (* Case: Some peer in the quorum has already committed up to the reported LSN. *)
+      destruct Hsomecmted as (nidx & b & Hfalse & ->).
+      unshelve epose proof (lookup_weaken _ aocm _ _ Hfalse _) as Hnidx.
+      { apply map_filter_subseteq. }
+      iDestruct (big_sepM2_dom with "Haocm") as %Hdom.
+      subst aocmq.
+      apply map_lookup_filter_Some_1_2 in Hfalse.
+      subst nidpeersq.
+      rewrite elem_of_dom /= in Hfalse.
+      destruct Hfalse as [lsncmted Hlsncmted].
+      subst lsnpeersq.
+      rewrite map_lookup_filter_Some /= in Hlsncmted.
+      destruct Hlsncmted as [Hlsncmted Hlenge].
+      iDestruct (big_sepM2_lookup with "Haocm") as "Hcmtedpeer".
+      { apply Hlsncmted. }
+      { apply Hnidx. }
+      iDestruct "Hcmtedpeer" as (logx) "[Hlogx %Hlenlogx]".
+      iDestruct (safe_ledger_above_weaken (take (uint.nat lsn) logx) with "Hlogx") as "Hcmted'".
+      { apply prefix_take. }
+      iFrame "Hcmted'".
+      iPureIntro.
+      rewrite length_take.
+      lia.
+    }
+    (* Case: All peers in the quorum have accepted up to their reported LSNs. *)
+    rewrite map_not_Exists in Hallacpted.
+    set logc := take (uint.nat lsn) log.
+    iExists logc.
+    iSplit; last first.
+    { iPureIntro.
+      rewrite length_take.
+      apply elem_of_list_lookup_2 in Hlsn.
+      rewrite Hperm -Hlsns' in Hlsn.
+      apply elem_of_list_lookup_1 in Hlsn as [j Hlsn].
+      rewrite list_lookup_fmap in Hlsn.
+      destruct (map_to_list lsnpeers !! j) as [[nidy lsny] |] eqn:Hy; last done.
+      inv Hlsn.
+      apply elem_of_list_lookup_2, elem_of_map_to_list in Hy.
+      specialize (Hlelog _ _ Hy). simpl in Hlelog.
+      clear -Hlelog. word.
+    }
+    iExists (uint.nat termc).
+    iSplit; last done.
+    set nidsq := ({[nidme]} ∪ nidpeersq).
+    iExists nidme, nidsq.
+    iDestruct (accepted_proposal_lb_weaken logc with "Hacpted") as "Hacpted'".
+    { apply prefix_take. }
+    subst terml.
+    iFrame "Hacpted'".
+    iSplit.
+    { rewrite big_sepM2_alt.
+      iDestruct "Haocm" as "[%Hdom Haocm]".
+      iDestruct (big_sepM_dom_subseteq_difference _ _ nidpeersq with "Haocm") as
+        (m) "([%Hdomm %Hm] & Haocm' & _)".
+      { rewrite dom_map_zip_with -Hdom intersection_idemp_L.
+        apply subseteq_dom, map_filter_subseteq.
+      }
+      iApply (big_sepS_insert_2 with "[] []").
+      { by iFrame "Hacpted'". }
+      rewrite big_sepS_big_sepM.
+      iApply (big_sepM_impl_dom_eq with "Haocm'"); first done.
+      iIntros (nid [x a] lsnp Hxa Hlsnp) "!> Hacpt".
+      assert (Ha : aocmq !! nid = Some a).
+      { rewrite map_lookup_filter_Some.
+        split.
+        { pose proof (lookup_weaken _ _ _ _ Hxa Hm) as Hlookup.
+          rewrite map_lookup_zip_Some in Hlookup.
+          by destruct Hlookup as [_ ?].
+        }
+        by rewrite elem_of_dom.
+      }
+      specialize (Hallacpted _ _ Ha).
+      rewrite not_false_iff_true in Hallacpted.
+      subst a. simpl.
+      rewrite map_lookup_filter_Some /= in Hlsnp.
+      destruct Hlsnp as [Hlsnp Hgelsn].
+      rewrite map_subseteq_spec in Hm.
+      specialize (Hm _ _ Hxa).
+      rewrite map_lookup_zip_Some /= in Hm.
+      destruct Hm as [Hx _].
+      rewrite Hlsnp in Hx.
+      inv Hx.
+      iApply (accepted_proposal_length_lb_weaken with "Hacpt").
+      rewrite length_take.
+      clear -Hgelsn. lia.
+    }
+    iPureIntro.
+    split; last set_solver.
+    split.
+    { apply union_least; first set_solver.
+      trans (dom lsnpeers); [apply dom_filter_subseteq | set_solver].
+    }
+    rewrite /cquorum_size.
+    rewrite size_union; last first.
+    { clear -Hnids Hnidsne Hinclnids.
+      assert (nidpeersq ⊆ peers).
+      { subst nidpeersq lsnpeersq.
+        trans (dom lsnpeers); [apply dom_filter_subseteq | apply Hinclnids].
+      }
+      set_solver.
+    }
+    rewrite size_singleton.
+    set lsndrops := drop (uint.nat i) lsnsorts.
+    assert (Hlensorts : size nids / 2 ≤ length lsndrops).
+    { rewrite length_drop.
+      rewrite Hperm -Hlsns' length_fmap length_map_to_list.
+      rewrite word.unsigned_sub_nowrap; last word.
+      word.
+    }
+    rewrite -Hlsns' in Hperm.
+    (* Key to this proof: Obtain from [lsnsorts] an inversion [nlsorts] with
+    node IDs, allowing proof of the following [submseteq] relation. We might be
+    able to simplify the proof by eliminating the detour using [filter] to
+    define the node IDs quorum, but define it directly using the [nlsorts]. *)
+    apply Permutation_map_inv in Hperm as (nlsorts & Hnlsorts & Hperm).
+    set nldrops := drop (uint.nat i) nlsorts.
+    assert (Hincl : nldrops ⊆+ map_to_list lsnpeersq).
+    { apply NoDup_submseteq.
+      { subst nldrops.
+        apply (NoDup_suffix _ nlsorts); first apply suffix_drop.
+        rewrite -Hperm.
+        apply NoDup_map_to_list.
+      }
+      intros nlx Hnlx.
+      assert (Hinsorts : nlx ∈ nlsorts).
+      { apply (subseteq_drop (uint.nat i) nlsorts _ Hnlx). }
+      rewrite -Hperm in Hinsorts.
+      destruct nlx as [nidx lsnx].
+      rewrite elem_of_map_to_list in Hinsorts.
+      rewrite elem_of_map_to_list.
+      rewrite map_lookup_filter_Some /=.
+      split; first apply Hinsorts.
+      apply elem_of_list_lookup in Hnlx as [j Hnlx].
+      subst nldrops.
+      rewrite lookup_drop /= in Hnlx.
+      assert (lsnsorts !! (uint.nat i + j)%nat = Some lsnx) as Hlsnx.
+      { by rewrite Hnlsorts list_lookup_fmap Hnlx /=. }
+      unshelve epose proof (Hsorted _ _ _ _ _ Hlsn Hlsnx) as Hle; first lia.
+      word.
+    }
+    assert (Hsizele : length lsndrops ≤ length (map_to_list lsnpeersq).*2).
+    { apply submseteq_length in Hincl.
+      revert Hincl.
+      rewrite 2!length_drop Hnlsorts 2!length_fmap.
+      word.
+    }
+    subst nidpeersq.
+    rewrite length_fmap length_map_to_list in Hsizele.
+    rewrite size_dom.
+    clear -Hsizele Hlensorts.
+    word.
+  Qed.
+
+End push.
 
 Section program.
   Context `{!heapGS Σ, !paxos_ghostG Σ}.
