src/program_proof/tulip/program/quorum.v
@@ -1,0 +1,24 @@
+From Perennial.program_proof.tulip Require Import prelude.
+From Goose.github_com.mit_pdos.tulip Require Import quorum.
+
+Section cquorum.
+  Context `{!heapGS Σ}.
+
+  Theorem wp_ClassicQuorum (n : u64) :
+    0 < uint.Z n ->
+    {{{ True }}}
+      ClassicQuorum #n
+    {{{ (x : u64), RET #x; ⌜uint.Z n / 2 < uint.Z x ≤ uint.Z n⌝ }}}.
+  Proof.
+    (*@ func ClassicQuorum(n uint64) uint64 {                                   @*)
+    (*@     // floor(n / 2) + 1                                                 @*)
+    (*@     return n / 2 + 1                                                    @*)
+    (*@ }                                                                       @*)
+    iIntros (Hgz Φ) "_ HΦ".
+    wp_rec. wp_pures.
+    iApply "HΦ".
+    iPureIntro.
+    word.
+  Qed.
+
+End cquorum.
