src/program_proof/tulip/program/util/sort.v
@@ -1,0 +1,34 @@
+From Perennial.program_proof.tulip Require Import prelude.
+From Goose.github_com.mit_pdos.tulip Require Import util.
+
+Definition sorted_u64 (ns : list u64) :=
+  ∀ i j x y, (i ≤ j)%nat -> ns !! i = Some x -> ns !! j = Some y -> uint.Z x ≤ uint.Z y.
+
+Section sort.
+  Context `{!heapGS Σ}.
+
+  Theorem wp_Sort (nsP : Slice.t) (ns : list u64) :
+    {{{ own_slice nsP uint64T (DfracOwn 1) ns }}}
+      Sort (to_val nsP)
+    {{{ (ns' : list u64), RET #(); 
+        own_slice nsP uint64T (DfracOwn 1) ns' ∗ ⌜sorted_u64 ns' ∧ ns' ≡ₚ ns⌝
+    }}}.
+  Proof.
+    (*@ func Sort(ns []uint64) {                                                @*)
+    (*@     // NB: Follow the proof of wrbuf.sortEntsByKey                      @*)
+    (*@     var i uint64 = 1                                                    @*)
+    (*@     for i < uint64(len(ns)) {                                           @*)
+    (*@         var j uint64 = i                                                @*)
+    (*@         for j > 0 {                                                     @*)
+    (*@             if ns[j - 1] <= ns[j] {                                     @*)
+    (*@                 break                                                   @*)
+    (*@             }                                                           @*)
+    (*@             swap(ns, j - 1, j)                                          @*)
+    (*@             j--                                                         @*)
+    (*@         }                                                               @*)
+    (*@         i++                                                             @*)
+    (*@     }                                                                   @*)
+    (*@ }                                                                       @*)
+  Admitted.
+
+End sort.
